test/auto_test.lean
@@ -1,6 +1,11 @@
--- import ..src.struct_tact
+import ..src.struct_tact
 
--- @[auto] inductive rel : nat → Type
--- | a : rel 0
--- | b : rel 1
--- | c : rel 2
+@[auto] inductive rel : nat → Type
+| a : rel 0
+| b : rel 1
+| c : rel 2
+
+lemma test_1 : rel 2 :=
+begin
+    auto,
+end
